Setlec/Kernel/CheckerS.lean
@@ -219,7 +219,7 @@ def checkEtaThmF (fe : FEnv) (T ctorName : Name) (lps : List Name)
       | some (.defnInfo cvmj _ _) => cvmj.levelParams == lps
       | _ => false) &&
     (match tcv.type.stripPis (nP + 1), cvmT.type.stripPis nP with
-     | some (sbinders, sbody), some (tbindersM, _) =>
+     | some (sbinders, sbody), some (tbindersM, tbodyM) =>
        domsMatchAux (fun _ e => e) sbinders tbindersM 0 0 nP &&
        (match sbinders[nP]? with
         | some (_, xdom, _) =>
@@ -227,7 +227,7 @@ def checkEtaThmF (fe : FEnv) (T ctorName : Name) (lps : List Name)
             ((List.range nP).map fun k => Expr.bvar (nP - 1 - k))
         | none => false) &&
        (match sbody with
-        | .app (.app (.app (.const c [_ℓ]) tySlot) lhsC) rhsC =>
+        | .app (.app (.app (.const c [ℓA]) tySlot) lhsC) rhsC =>
           c == eqName && lhsC == Expr.bvar 0 &&
           tySlot == Expr.mkAppN (.const (T.str "_model") (lps.map .param))
             ((List.range nP).map fun k => Expr.bvar (nP - k)) &&
@@ -237,7 +237,8 @@ def checkEtaThmF (fe : FEnv) (T ctorName : Name) (lps : List Name)
              (List.range nF).map fun j => Expr.mkAppN
                (.const (projModelName T j) (lps.map .param))
                (((List.range nP).map fun k => Expr.bvar (nP - k)) ++
-                [Expr.bvar 0]))
+                [Expr.bvar 0])) &&
+          tbodyM == Expr.sort ℓA
         | _ => false)
      | _, _ => false)
   | _, _, _, _ => false
@@ -251,7 +252,7 @@ def checkUnitThmF (fe : FEnv) (T : Name) (lps : List Name)
     eqStored == eqA && tcv.levelParams == lps &&
     cvmT.levelParams == lps &&
     (match tcv.type.stripPis (nP + 2), cvmT.type.stripPis nP with
-     | some (sbinders, sbody), some (tbindersM, _) =>
+     | some (sbinders, sbody), some (tbindersM, tbodyM) =>
        domsMatchAux (fun _ e => e) sbinders tbindersM 0 0 nP &&
        (match sbinders[nP]? with
         | some (_, xdom, _) =>
@@ -264,10 +265,11 @@ def checkUnitThmF (fe : FEnv) (T : Name) (lps : List Name)
             ((List.range nP).map fun k => Expr.bvar (nP - k))
         | none => false) &&
        (match sbody with
-        | .app (.app (.app (.const c [_ℓ]) tySlot) lhsC) rhsC =>
+        | .app (.app (.app (.const c [ℓA]) tySlot) lhsC) rhsC =>
           c == eqName && lhsC == Expr.bvar 1 && rhsC == Expr.bvar 0 &&
           tySlot == Expr.mkAppN (.const (T.str "_model") (lps.map .param))
-            ((List.range nP).map fun k => Expr.bvar (nP + 1 - k))
+            ((List.range nP).map fun k => Expr.bvar (nP + 1 - k)) &&
+          tbodyM == Expr.sort ℓA
         | _ => false)
      | _, _ => false)
   | _, _, _ => false
